project/Big_Small_Eq.v
@@ -1,0 +1,10 @@
+Require Import Imp_Syntax.
+Require Import Imp_Big_Step.
+Require Import Imp_Small_Step.
+Require Import Coq.Strings.String.
+
+Definition State := string -> (option nat).
+
+Theorem Big_Small_Equiv : forall (P : Program) (S : State),
+  (BigStepR (B_PgmConf P) (B_StateConf S)) <-> (SmallStepR (S_PgmConf P) (S_BlkConf EmptyBlk S)).
+Admitted.
