project/Imp_Big_Step.v
@@ -1,0 +1,20 @@
+Require Import Imp_Syntax.
+Require Import Coq.Strings.String.
+
+Definition State := string -> (option nat).
+
+Inductive BigConfig : Type := 
+  | B_AExpConf : AExp -> State -> BigConfig
+  | B_NatConf : nat -> BigConfig
+  | B_BExpConf : BExp -> State -> BigConfig
+  | B_BoolConf : bool -> BigConfig
+  | B_StmtConf : Statement -> State -> BigConfig
+  | B_BlkConf : Block -> State -> BigConfig
+  | B_StateConf : State -> BigConfig
+  | B_PgmConf : Program -> BigConfig.
+
+
+Inductive BigStepR : BigConfig -> BigConfig -> Prop :=
+  | Block : forall (S : Statement) (Sigma Sigma' : State),
+      BigStepR (B_StmtConf S Sigma) (B_StateConf Sigma') ->
+      BigStepR (B_BlkConf (Blk S) Sigma) (B_StateConf Sigma').
