project/Imp_Small_Step.v
@@ -1,0 +1,16 @@
+Require Import Imp_Syntax.
+Require Import Coq.Strings.String.
+
+Definition State := string -> (option nat).
+
+Inductive SmallConfig : Type := 
+  | S_AExpConf : AExp -> State -> SmallConfig
+  | S_BExpConf : BExp -> State -> SmallConfig
+  | S_StmtConf : Statement -> State -> SmallConfig
+  | S_BlkConf : Block -> State -> SmallConfig
+  | S_PgmConf : Program -> SmallConfig.
+
+
+Inductive SmallStepR : SmallConfig -> SmallConfig -> Prop :=
+  | Block : forall (S : Statement) (Sigma : State),
+      SmallStepR (S_BlkConf (Blk S) Sigma) (S_StmtConf S Sigma).
