project/Imp_Small_step.v
@@ -1,0 +1,16 @@
+Require Import Imp_Syntax.
+Require Import Coq.Strings.String.
+
+Definition State := string -> (option nat).
+
+Inductive SmallConfig : Type := 
+  | AExpConf : AExp -> State -> SmallConfig
+  | BExpConf : BExp -> State -> SmallConfig
+  | StmtConf : Statement -> State -> SmallConfig
+  | BlkConf : Block -> State -> SmallConfig
+  | PgmConf : Program -> SmallConfig.
+
+
+Inductive SmallStepR : SmallConfig -> SmallConfig -> Prop :=
+  | Block : forall (S : Statement) (Sigma : State),
+      SmallStepR (BlkConf (Blk S) Sigma) (StmtConf S Sigma).
