project/Imp_Syntax.v
@@ -1,0 +1,26 @@
+Require Import Coq.Strings.String.
+
+Inductive AExp : Type :=
+  | ANum : nat -> AExp
+  | APlus : AExp -> AExp -> AExp
+  | ADiv : AExp -> AExp -> AExp
+  | AId : string -> AExp.
+
+Inductive BExp : Type :=
+  | BTrue : BExp
+  | BFalse : BExp
+  | BLe : AExp -> AExp -> BExp
+  | BNot : BExp -> BExp
+  | BAnd : BExp -> BExp -> BExp.
+
+Inductive Block : Type :=
+  | EmptyBlk : Block
+  | Blk : Statement -> Block
+with Statement : Type :=
+  | Assignment : string -> AExp -> Statement
+  | Seq : Statement -> Statement -> Statement
+  | IfElse : BExp -> Block -> Block -> Statement
+  | While : BExp -> Block -> Statement.
+
+Inductive Program : Type :=
+  | Pgm : list string -> Statement -> Program.
